<?xml version="1.0" encoding="UTF-8"?>
<!DOCTYPE rdf:RDF [
	<!ENTITY cmns-av "https://www.omg.org/spec/Commons/AnnotationVocabulary/">
	<!ENTITY cmns-cls "https://www.omg.org/spec/Commons/Classifiers/">
	<!ENTITY cmns-col "https://www.omg.org/spec/Commons/Collections/">
	<!ENTITY cmns-dsg "https://www.omg.org/spec/Commons/Designators/">
	<!ENTITY cmns-dt "https://www.omg.org/spec/Commons/DatesAndTimes/">
	<!ENTITY cmns-pts "https://www.omg.org/spec/Commons/PartiesAndSituations/">
	<!ENTITY cmns-qtu "https://www.omg.org/spec/Commons/QuantitiesAndUnits/">
	<!ENTITY dct "http://purl.org/dc/terms/">
	<!ENTITY oe2022-iem "https://tw.rpi.edu/ontology-engineering/oe2022/indoor-environment-manager/">
	<!ENTITY owl "http://www.w3.org/2002/07/owl#">
	<!ENTITY rdf "http://www.w3.org/1999/02/22-rdf-syntax-ns#">
	<!ENTITY rdfs "http://www.w3.org/2000/01/rdf-schema#">
	<!ENTITY skos "http://www.w3.org/2004/02/skos/core#">
	<!ENTITY xsd "http://www.w3.org/2001/XMLSchema#">
]>
<rdf:RDF xml:base="https://tw.rpi.edu/ontology-engineering/oe2022/indoor-environment-manager/"
	xmlns:cmns-av="https://www.omg.org/spec/Commons/AnnotationVocabulary/"
	xmlns:cmns-cls="https://www.omg.org/spec/Commons/Classifiers/"
	xmlns:cmns-col="https://www.omg.org/spec/Commons/Collections/"
	xmlns:cmns-dsg="https://www.omg.org/spec/Commons/Designators/"
	xmlns:cmns-dt="https://www.omg.org/spec/Commons/DatesAndTimes/"
	xmlns:cmns-pts="https://www.omg.org/spec/Commons/PartiesAndSituations/"
	xmlns:cmns-qtu="https://www.omg.org/spec/Commons/QuantitiesAndUnits/"
	xmlns:dct="http://purl.org/dc/terms/"
	xmlns:oe2022-iem="https://tw.rpi.edu/ontology-engineering/oe2022/indoor-environment-manager/"
	xmlns:owl="http://www.w3.org/2002/07/owl#"
	xmlns:rdf="http://www.w3.org/1999/02/22-rdf-syntax-ns#"
	xmlns:rdfs="http://www.w3.org/2000/01/rdf-schema#"
	xmlns:skos="http://www.w3.org/2004/02/skos/core#"
	xmlns:xsd="http://www.w3.org/2001/XMLSchema#">
	
	<owl:Ontology rdf:about="https://tw.rpi.edu/ontology-engineering/oe2022/indoor-environment-manager/">
		<rdfs:label>Indoor Environment Manager Ontology</rdfs:label>
		<dct:abstract>The goal of this ontology is to assist occupants to improve indoor environmental quality (IEQ) and minimize energy use in a small room. This process considers components of the room that can change environmental conditions or allow the outdoor environment to affect the indoor environment, as well as sensors to record various environment attributes, and the occupants&apos; comfort ranges.</dct:abstract>
		<dct:creator>Gabriel Jacoby-Cooper</dct:creator>
		<dct:creator>Jihoon Chung</dct:creator>
		<dct:creator>Kelsey Rook</dct:creator>
		<dct:modified>November 18, 2022</dct:modified>
		<dct:publisher>IEQ Management System</dct:publisher>
		<owl:imports rdf:resource="https://www.omg.org/spec/Commons/AnnotationVocabulary/"/>
		<owl:imports rdf:resource="https://www.omg.org/spec/Commons/Classifiers/"/>
		<owl:imports rdf:resource="https://www.omg.org/spec/Commons/Collections/"/>
		<owl:imports rdf:resource="https://www.omg.org/spec/Commons/DatesAndTimes/"/>
		<owl:imports rdf:resource="https://www.omg.org/spec/Commons/Designators/"/>
		<owl:imports rdf:resource="https://www.omg.org/spec/Commons/PartiesAndSituations/"/>
		<owl:versionIRI>https://tw.rpi.edu/ontology-engineering/oe2022/indoor-environment-manager/</owl:versionIRI>
	</owl:Ontology>
	
	<owl:AnnotationProperty rdf:about="&dct;bibliographicCitation">
	</owl:AnnotationProperty>
	
	<owl:AnnotationProperty rdf:about="&dct;creator">
	</owl:AnnotationProperty>
	
	<owl:AnnotationProperty rdf:about="&owl;versionIRI">
	</owl:AnnotationProperty>
	
	<owl:Class rdf:about="&oe2022-iem;AirConditioning">
		<rdfs:subClassOf rdf:resource="&oe2022-iem;HeatingVentilationAndAirConditioningEquipment"/>
		<rdfs:subClassOf>
			<owl:Restriction>
				<owl:onProperty rdf:resource="&oe2022-iem;isControlledBy"/>
				<owl:onClass rdf:resource="&oe2022-iem;Thermostat"/>
				<owl:qualifiedCardinality rdf:datatype="&xsd;nonNegativeInteger">1</owl:qualifiedCardinality>
			</owl:Restriction>
		</rdfs:subClassOf>
		<rdfs:label>air conditioning</rdfs:label>
		<dct:source>&quot;Air conditioning&quot;, ASHRAE Terminology, 2022. [Online] Available: https://terminology.ashrae.org/?term=air+conditioning</dct:source>
		<skos:definition>equipment, distribution systems, and terminals that controlits temperature, humidity, cleanliness, and distribution in a building in order to meet the requirements of a conditioned space</skos:definition>
	</owl:Class>
	
	<owl:NamedIndividual rdf:about="&oe2022-iem;AirQuality">
		<rdf:type rdf:resource="&owl;Class"/>
		<rdf:type rdf:resource="&cmns-qtu;QuantityKind"/>
		<rdfs:subClassOf rdf:resource="&oe2022-iem;IndoorEnvironmentalQuality"/>
		<rdfs:label>air quality</rdfs:label>
		<dct:bibliographicCitation>D. Heinzerling, S. Schiavon, T. Webster, and E. Arens, &apos;Indoor Environmental Quality Assessment models: A literature review and a proposed weighting and classification scheme,&apos; Building and Environment, vol. 70, pp. 210 to 222, 2013.  P. Antoniadou and A. M. Papadopoulos, &apos;Occupants&apos; thermal comfort: State of the art and the prospects of personalized assessment in office buildings,&apos; Energy and Buildings, vol. 153, pp. 136 to 149, 2017.</dct:bibliographicCitation>
		<dct:source>&apos;Center for Science Education,&apos; What Is Air Quality? [Online]. Available: https://scied.ucar.edu/learning-zone/air-quality/what-is-air-quality. [Accessed: 22-Sep-2022].</dct:source>
		<owl:disjointWith rdf:resource="&oe2022-iem;ThermalComfort"/>
		<skos:definition>synthesis of various physical measurements of properties of air that threaten human health</skos:definition>
	</owl:NamedIndividual>
	
	<owl:NamedIndividual rdf:about="&oe2022-iem;AirQualityIndex">
		<rdf:type rdf:resource="&cmns-qtu;MeasurementUnit"/>
		<rdfs:label>air quality index</rdfs:label>
		<skos:definition>measurement that combines other meaurements of properties of air to indicate the level of danger to human health</skos:definition>
	</owl:NamedIndividual>
	
	<owl:NamedIndividual rdf:about="&oe2022-iem;AirSpeed">
		<rdf:type rdf:resource="&cmns-qtu;QuantityKind"/>
		<rdfs:label>air speed</rdfs:label>
		<skos:definition>the rate of air movement at a point, without regard to direction.</skos:definition>
	</owl:NamedIndividual>
	
	<owl:NamedIndividual rdf:about="&oe2022-iem;Closed">
		<rdf:type rdf:resource="&oe2022-iem;ComponentState"/>
		<rdfs:label>closed</rdfs:label>
		<skos:definition>the condition of not being open</skos:definition>
	</owl:NamedIndividual>
	
	<owl:Class rdf:about="&oe2022-iem;ComponentState">
		<rdfs:subClassOf rdf:resource="&cmns-cls;Classifier"/>
		<rdfs:label>component state</rdfs:label>
		<skos:definition>the state of an object in a room that can be used to alter relevant indoor environment quality parameters</skos:definition>
	</owl:Class>
	
	<owl:Class rdf:about="&oe2022-iem;CurrentIndoorEnvironment">
		<rdfs:subClassOf rdf:resource="&oe2022-iem;IndoorEnvironment"/>
		<rdfs:label>current indoor environment</rdfs:label>
		<skos:definition>a collection of indoor environmental parameters before environmental attributes affect the indoor environment</skos:definition>
	</owl:Class>
	
	<owl:NamedIndividual rdf:about="&oe2022-iem;DaylightIntensity">
		<rdf:type rdf:resource="&cmns-qtu;QuantityKind"/>
		<rdfs:label>daylight intensity</rdfs:label>
		<skos:definition>a quantitative attribute that affects daylight intensity in a local environment</skos:definition>
	</owl:NamedIndividual>
	
	<owl:Class rdf:about="&oe2022-iem;Dehumidifier">
		<rdfs:subClassOf rdf:resource="&oe2022-iem;PowerConsumingComponent"/>
		<rdfs:label>dehumidifier</rdfs:label>
		<dct:source>&quot;Dehumidifier&quot;, ASHRAE Terminology, 2022. [Online] Available: https://terminology.ashrae.org/?term=dehumidifier</dct:source>
		<skos:definition>an air cooler or an absorption or adsorption device used for lowering moisture content</skos:definition>
	</owl:Class>
	
	<owl:Class rdf:about="&oe2022-iem;DeltaDefinedEnvironment">
		<rdfs:subClassOf rdf:resource="&oe2022-iem;Environment"/>
		<rdfs:subClassOf>
			<owl:Class>
				<owl:unionOf rdf:parseType="Collection">
					<owl:Class>
						<owl:complementOf>
							<owl:Restriction>
								<owl:onProperty rdf:resource="&oe2022-iem;hasAirSpeedValue"/>
								<owl:someValuesFrom rdf:resource="&xsd;integer"/>
							</owl:Restriction>
						</owl:complementOf>
					</owl:Class>
					<owl:Restriction>
						<owl:onProperty rdf:resource="&oe2022-iem;hasAirSpeedSign"/>
						<owl:someValuesFrom rdf:resource="&oe2022-iem;Sign"/>
					</owl:Restriction>
				</owl:unionOf>
			</owl:Class>
		</rdfs:subClassOf>
		<rdfs:subClassOf>
			<owl:Class>
				<owl:unionOf rdf:parseType="Collection">
					<owl:Class>
						<owl:complementOf>
							<owl:Restriction>
								<owl:onProperty rdf:resource="&oe2022-iem;hasAirTemperatureValue"/>
								<owl:someValuesFrom rdf:resource="&xsd;integer"/>
							</owl:Restriction>
						</owl:complementOf>
					</owl:Class>
					<owl:Restriction>
						<owl:onProperty rdf:resource="&oe2022-iem;hasAirTemperatureSign"/>
						<owl:someValuesFrom rdf:resource="&oe2022-iem;Sign"/>
					</owl:Restriction>
				</owl:unionOf>
			</owl:Class>
		</rdfs:subClassOf>
		<rdfs:subClassOf>
			<owl:Class>
				<owl:unionOf rdf:parseType="Collection">
					<owl:Class>
						<owl:complementOf>
							<owl:Restriction>
								<owl:onProperty rdf:resource="&oe2022-iem;hasRelativeHumidityValue"/>
								<owl:someValuesFrom rdf:resource="&xsd;integer"/>
							</owl:Restriction>
						</owl:complementOf>
					</owl:Class>
					<owl:Restriction>
						<owl:onProperty rdf:resource="&oe2022-iem;hasRelativeHumiditySign"/>
						<owl:someValuesFrom rdf:resource="&oe2022-iem;Sign"/>
					</owl:Restriction>
				</owl:unionOf>
			</owl:Class>
		</rdfs:subClassOf>
		<rdfs:subClassOf>
			<owl:Restriction>
				<owl:onProperty rdf:resource="&oe2022-iem;hasAirSpeedSign"/>
				<owl:onClass rdf:resource="&oe2022-iem;Sign"/>
				<owl:minQualifiedCardinality rdf:datatype="&xsd;nonNegativeInteger">0</owl:minQualifiedCardinality>
			</owl:Restriction>
		</rdfs:subClassOf>
		<rdfs:subClassOf>
			<owl:Restriction>
				<owl:onProperty rdf:resource="&oe2022-iem;hasAirTemperatureSign"/>
				<owl:onClass rdf:resource="&oe2022-iem;Sign"/>
				<owl:minQualifiedCardinality rdf:datatype="&xsd;nonNegativeInteger">0</owl:minQualifiedCardinality>
			</owl:Restriction>
		</rdfs:subClassOf>
		<rdfs:subClassOf>
			<owl:Restriction>
				<owl:onProperty rdf:resource="&oe2022-iem;hasRelativeHumiditySign"/>
				<owl:onClass rdf:resource="&oe2022-iem;Sign"/>
				<owl:minQualifiedCardinality rdf:datatype="&xsd;nonNegativeInteger">0</owl:minQualifiedCardinality>
			</owl:Restriction>
		</rdfs:subClassOf>
		<rdfs:label>delta defined environment</rdfs:label>
		<skos:definition>any environment that happens to be defined in terms of effectiveness with respect to some other environment</skos:definition>
	</owl:Class>
	
	<owl:NamedIndividual rdf:about="&oe2022-iem;Energy">
		<rdf:type rdf:resource="&cmns-qtu;QuantityKind"/>
		<rdfs:label>energy</rdfs:label>
		<skos:definition>measurement of the ability of something to do work</skos:definition>
	</owl:NamedIndividual>
	
	<owl:Class rdf:about="&oe2022-iem;Environment">
		<rdfs:subClassOf>
			<owl:Restriction>
				<owl:onProperty rdf:resource="&oe2022-iem;hasAirQualityValue"/>
				<owl:maxQualifiedCardinality rdf:datatype="&xsd;nonNegativeInteger">1</owl:maxQualifiedCardinality>
				<owl:onDataRange>
					<rdfs:Datatype>
						<owl:onDatatype rdf:resource="&xsd;integer"/>
						<owl:withRestrictions rdf:parseType="Collection">
							<rdf:Description>
								<xsd:minInclusive rdf:datatype="&xsd;integer">0</xsd:minInclusive>
							</rdf:Description>
							<rdf:Description>
								<xsd:maxInclusive rdf:datatype="&xsd;integer">400</xsd:maxInclusive>
							</rdf:Description>
						</owl:withRestrictions>
					</rdfs:Datatype>
				</owl:onDataRange>
			</owl:Restriction>
		</rdfs:subClassOf>
		<rdfs:subClassOf>
			<owl:Restriction>
				<owl:onProperty rdf:resource="&oe2022-iem;hasAirSpeedValue"/>
				<owl:maxQualifiedCardinality rdf:datatype="&xsd;nonNegativeInteger">1</owl:maxQualifiedCardinality>
				<owl:onDataRange>
					<rdfs:Datatype>
						<owl:onDatatype rdf:resource="&xsd;integer"/>
						<owl:withRestrictions rdf:parseType="Collection">
							<rdf:Description>
								<xsd:minInclusive rdf:datatype="&xsd;integer">0</xsd:minInclusive>
							</rdf:Description>
							<rdf:Description>
								<xsd:maxInclusive rdf:datatype="&xsd;integer">30</xsd:maxInclusive>
							</rdf:Description>
						</owl:withRestrictions>
					</rdfs:Datatype>
				</owl:onDataRange>
			</owl:Restriction>
		</rdfs:subClassOf>
		<rdfs:subClassOf>
			<owl:Restriction>
				<owl:onProperty rdf:resource="&oe2022-iem;hasAirTemperatureValue"/>
				<owl:maxQualifiedCardinality rdf:datatype="&xsd;nonNegativeInteger">1</owl:maxQualifiedCardinality>
				<owl:onDataRange>
					<rdfs:Datatype>
						<owl:onDatatype rdf:resource="&xsd;integer"/>
						<owl:withRestrictions rdf:parseType="Collection">
							<rdf:Description>
								<xsd:minInclusive rdf:datatype="&xsd;integer">0</xsd:minInclusive>
							</rdf:Description>
							<rdf:Description>
								<xsd:maxInclusive rdf:datatype="&xsd;integer">104</xsd:maxInclusive>
							</rdf:Description>
						</owl:withRestrictions>
					</rdfs:Datatype>
				</owl:onDataRange>
			</owl:Restriction>
		</rdfs:subClassOf>
		<rdfs:subClassOf>
			<owl:Restriction>
				<owl:onProperty rdf:resource="&oe2022-iem;hasDaylightIntensityValue"/>
				<owl:maxQualifiedCardinality rdf:datatype="&xsd;nonNegativeInteger">1</owl:maxQualifiedCardinality>
				<owl:onDataRange>
					<rdfs:Datatype>
						<owl:onDatatype rdf:resource="&xsd;integer"/>
						<owl:withRestrictions rdf:parseType="Collection">
							<rdf:Description>
								<xsd:minInclusive rdf:datatype="&xsd;integer">0</xsd:minInclusive>
							</rdf:Description>
							<rdf:Description>
								<xsd:maxInclusive rdf:datatype="&xsd;integer">10000</xsd:maxInclusive>
							</rdf:Description>
						</owl:withRestrictions>
					</rdfs:Datatype>
				</owl:onDataRange>
			</owl:Restriction>
		</rdfs:subClassOf>
		<rdfs:subClassOf>
			<owl:Restriction>
				<owl:onProperty rdf:resource="&oe2022-iem;hasRelativeHumidityValue"/>
				<owl:maxQualifiedCardinality rdf:datatype="&xsd;nonNegativeInteger">1</owl:maxQualifiedCardinality>
				<owl:onDataRange>
					<rdfs:Datatype>
						<owl:onDatatype rdf:resource="&xsd;integer"/>
						<owl:withRestrictions rdf:parseType="Collection">
							<rdf:Description>
								<xsd:minInclusive rdf:datatype="&xsd;integer">0</xsd:minInclusive>
							</rdf:Description>
							<rdf:Description>
								<xsd:maxInclusive rdf:datatype="&xsd;integer">100</xsd:maxInclusive>
							</rdf:Description>
						</owl:withRestrictions>
					</rdfs:Datatype>
				</owl:onDataRange>
			</owl:Restriction>
		</rdfs:subClassOf>
		<rdfs:label>environment</rdfs:label>
		<dct:source>&quot;Environment&quot;, ASHRAE Terminology, 2022. [Online] Available: https://terminology.ashrae.org/?term=environment</dct:source>
		<skos:definition>all of the elements over which a designer has no control and that affect a system and its input or output</skos:definition>
	</owl:Class>
	
	<owl:Class rdf:about="&oe2022-iem;Fan">
		<rdfs:subClassOf rdf:resource="&oe2022-iem;PowerConsumingComponent"/>
		<rdfs:label>fan</rdfs:label>
		<dct:bibliographicCitation>J. Xie, H. Li, C. Li, J. Zhang, and M. Luo, &apos;Review on occupant-centric thermal comfort sensing, predicting, and controlling,&apos; Energy and Buildings, vol. 226, p. 110392, 2020.</dct:bibliographicCitation>
		<dct:source>&quot;Fan,&quot; Merriam-Webster.com, 2022. [Online]. Available: https://www.merriam-webster.com/dictionary/fan</dct:source>
		<skos:definition>piece of equipment that can increase air speed</skos:definition>
	</owl:Class>
	
	<owl:Class rdf:about="&oe2022-iem;HeatingVentilationAndAirConditioningEquipment">
		<rdfs:subClassOf rdf:resource="&oe2022-iem;PowerConsumingComponent"/>
		<rdfs:label>heating, ventilation, and air conditioning equipment</rdfs:label>
		<dct:bibliographicCitation>J. Xie, H. Li, C. Li, J. Zhang, and M. Luo, &apos;Review on occupant-centric thermal comfort sensing, predicting, and controlling,&apos; Energy and Buildings, vol. 226, p. 110392, 2020.</dct:bibliographicCitation>
		<dct:source>&quot;HVAC system&quot;, ASHRAE Terminology, 2022. [Online] Available: https://xp20.ashrae.org/terminology/index.php?term=hvac&amp;submit=Search</dct:source>
		<skos:definition>the equipment, distribution systems, and terminals that provide, either collectively or individually, the processes of heating, ventilating, or air conditioning to a building or portion of a building</skos:definition>
		<cmns-av:acronym>HVAC</cmns-av:acronym>
	</owl:Class>
	
	<owl:Class rdf:about="&oe2022-iem;IdealIndoorEnvironment">
		<rdfs:subClassOf rdf:resource="&oe2022-iem;DeltaDefinedEnvironment"/>
		<rdfs:subClassOf rdf:resource="&oe2022-iem;IndoorEnvironment"/>
		<rdfs:label>ideal indoor environment</rdfs:label>
		<skos:definition>a collection of indoor environmental parameters that represent the target towards which actions should make progress</skos:definition>
	</owl:Class>
	
	<owl:Class rdf:about="&oe2022-iem;IndoorEnvironment">
		<rdfs:subClassOf rdf:resource="&oe2022-iem;Environment"/>
		<rdfs:subClassOf>
			<owl:Restriction>
				<owl:onProperty rdf:resource="&oe2022-iem;hasAirQualityValue"/>
				<owl:onDataRange>
					<rdfs:Datatype>
						<owl:onDatatype rdf:resource="&xsd;integer"/>
						<owl:withRestrictions rdf:parseType="Collection">
							<rdf:Description>
								<xsd:maxInclusive rdf:datatype="&xsd;integer">400</xsd:maxInclusive>
							</rdf:Description>
						</owl:withRestrictions>
					</rdfs:Datatype>
				</owl:onDataRange>
				<owl:qualifiedCardinality rdf:datatype="&xsd;nonNegativeInteger">0</owl:qualifiedCardinality>
			</owl:Restriction>
		</rdfs:subClassOf>
		<rdfs:subClassOf>
			<owl:Restriction>
				<owl:onProperty rdf:resource="&oe2022-iem;hasDaylightIntensityValue"/>
				<owl:onDataRange>
					<rdfs:Datatype>
						<owl:onDatatype rdf:resource="&xsd;integer"/>
						<owl:withRestrictions rdf:parseType="Collection">
							<rdf:Description>
								<xsd:minInclusive rdf:datatype="&xsd;integer">0</xsd:minInclusive>
							</rdf:Description>
							<rdf:Description>
								<xsd:maxInclusive rdf:datatype="&xsd;integer">10000</xsd:maxInclusive>
							</rdf:Description>
						</owl:withRestrictions>
					</rdfs:Datatype>
				</owl:onDataRange>
				<owl:qualifiedCardinality rdf:datatype="&xsd;nonNegativeInteger">0</owl:qualifiedCardinality>
			</owl:Restriction>
		</rdfs:subClassOf>
		<rdfs:label>indoor environment</rdfs:label>
		<dct:source>&quot;Environment&quot;, ASHRAE Terminology, 2022. [Online] Available: https://terminology.ashrae.org/?term=environment</dct:source>
		<skos:definition>all of the indoor elements over which a designer has no control and that affect a system and its input or output</skos:definition>
	</owl:Class>
	
	<owl:Class rdf:about="&oe2022-iem;IndoorEnvironmentalQuality">
		<rdfs:label>indoor environmental quality</rdfs:label>
		<dct:source>&quot;Indoor environmental quality&quot;, ASHRAE Terminology, 2022. [Online]. Available: https://xp20.ashrae.org/terminology/index.php?term=thermal&amp;submit=Search</dct:source>
		<rdfs:seeAlso>D. Heinzerling, S. Schiavon, T. Webster, and E. Arens, &apos;Indoor Environmental Quality Assessment models: A literature review and a proposed weighting and classification scheme,&apos; Building and Environment, vol. 70, pp. 210 to 222, 2013.</rdfs:seeAlso>
		<skos:definition>a perceived indoor experience of the building indoor including thermal comfort, indoor air quality, lighting, acoustics, and control systems</skos:definition>
	</owl:Class>
	
	<owl:NamedIndividual rdf:about="&oe2022-iem;Kelvin">
		<rdf:type rdf:resource="&cmns-qtu;MeasurementUnit"/>
		<rdfs:label>kelvin</rdfs:label>
		<dct:source>https://ucum.org/ucum.html#section-Base-Units</dct:source>
		<rdfs:seeAlso rdf:resource="https://www.nist.gov/pml/owm/si-units-temperature"/>
		<skos:definition>base unit of temperature that is defined by taking the fixed numerical value of the Boltzmann constant k to be 1.380 649 *10e(-23) when expressed in the unit J Ke(-1), which is equal to kg me(2) se(-2) Ke(-1)</skos:definition>
		<cmns-av:explanatoryNote>The temperature 0 K is commonly referred to as &apos;absolute zero.&apos; On the widely used Celsius temperature scale, water freezes at 0 C and boils at about 100 C. One Celsius degree is an interval of 1 K, and zero degrees Celsius is 273.15 K. An interval of one Celsius degree corresponds to an interval of 1.8 Fahrenheit degrees on the Fahrenheit temperature scale.</cmns-av:explanatoryNote>
		<cmns-av:symbol>K</cmns-av:symbol>
	</owl:NamedIndividual>
	
	<owl:NamedIndividual rdf:about="&oe2022-iem;Kilogram">
		<rdf:type rdf:resource="&cmns-qtu;MeasurementUnit"/>
		<rdfs:label>kilogram</rdfs:label>
		<dct:source>https://ucum.org/ucum.html#section-Base-Units</dct:source>
		<rdfs:seeAlso rdf:resource="https://www.nist.gov/si-redefinition/kilogram"/>
		<skos:definition>conversion-based unit of mass</skos:definition>
		<skos:note>Note that in the International System of Units (SI), the kilogram is considered the base unit rather than the gram, which is the base unit in the UCUM.</skos:note>
		<cmns-av:symbol>kg</cmns-av:symbol>
	</owl:NamedIndividual>
	
	<owl:NamedIndividual rdf:about="&oe2022-iem;KilowattHour">
		<rdf:type rdf:resource="&cmns-qtu;MeasurementUnit"/>
		<rdfs:label>kilowatt-hour</rdfs:label>
		<skos:definition>measure of electrical energy equivalent to a power consumption of 1,000 watts for 1 hour</skos:definition>
	</owl:NamedIndividual>
	
	<owl:NamedIndividual rdf:about="&oe2022-iem;MetersPerSecond">
		<rdf:type rdf:resource="&cmns-qtu;MeasurementUnit"/>
		<rdfs:label>meter per second</rdfs:label>
		<skos:definition>measure of speed equipvalent to the moved meters for 1 second</skos:definition>
	</owl:NamedIndividual>
	
	<owl:NamedIndividual rdf:about="&oe2022-iem;Negative">
		<rdf:type rdf:resource="&oe2022-iem;Sign"/>
		<rdfs:label>negative</rdfs:label>
		<skos:definition>minus sign that indicates how attributes affects the environment in a negative way</skos:definition>
	</owl:NamedIndividual>
	
	<owl:Class rdf:about="&oe2022-iem;NonPowerConsumingComponent">
		<rdfs:subClassOf rdf:resource="&oe2022-iem;RoomComponent"/>
		<rdfs:label>non-power consuming component</rdfs:label>
		<owl:disjointWith rdf:resource="&oe2022-iem;PowerConsumingComponent"/>
		<skos:definition>room component that does not consume energy</skos:definition>
	</owl:Class>
	
	<owl:Class rdf:about="&oe2022-iem;Occupant">
		<rdfs:subClassOf rdf:resource="&cmns-pts;PartyRole"/>
		<rdfs:subClassOf>
			<owl:Restriction>
				<owl:onProperty rdf:resource="&cmns-pts;isPlayedBy"/>
				<owl:onClass rdf:resource="&oe2022-iem;Person"/>
				<owl:qualifiedCardinality rdf:datatype="&xsd;nonNegativeInteger">1</owl:qualifiedCardinality>
			</owl:Restriction>
		</rdfs:subClassOf>
		<rdfs:subClassOf>
			<owl:Restriction>
				<owl:onProperty rdf:resource="&oe2022-iem;hasAirSpeedComfortRangeLowerBound"/>
				<owl:onDataRange rdf:resource="&xsd;integer"/>
				<owl:qualifiedCardinality rdf:datatype="&xsd;nonNegativeInteger">1</owl:qualifiedCardinality>
			</owl:Restriction>
		</rdfs:subClassOf>
		<rdfs:subClassOf>
			<owl:Restriction>
				<owl:onProperty rdf:resource="&oe2022-iem;hasAirSpeedComfortRangeUpperBound"/>
				<owl:onDataRange rdf:resource="&xsd;integer"/>
				<owl:qualifiedCardinality rdf:datatype="&xsd;nonNegativeInteger">1</owl:qualifiedCardinality>
			</owl:Restriction>
		</rdfs:subClassOf>
		<rdfs:subClassOf>
			<owl:Restriction>
				<owl:onProperty rdf:resource="&oe2022-iem;hasAirTemperatureComfortRangeLowerBound"/>
				<owl:onDataRange rdf:resource="&xsd;integer"/>
				<owl:qualifiedCardinality rdf:datatype="&xsd;nonNegativeInteger">1</owl:qualifiedCardinality>
			</owl:Restriction>
		</rdfs:subClassOf>
		<rdfs:subClassOf>
			<owl:Restriction>
				<owl:onProperty rdf:resource="&oe2022-iem;hasAirTemperatureComfortRangeUpperBound"/>
				<owl:onDataRange rdf:resource="&xsd;integer"/>
				<owl:qualifiedCardinality rdf:datatype="&xsd;nonNegativeInteger">1</owl:qualifiedCardinality>
			</owl:Restriction>
		</rdfs:subClassOf>
		<rdfs:subClassOf>
			<owl:Restriction>
				<owl:onProperty rdf:resource="&oe2022-iem;hasRelativeHumidityComfortRangeLowerBound"/>
				<owl:onDataRange rdf:resource="&xsd;integer"/>
				<owl:qualifiedCardinality rdf:datatype="&xsd;nonNegativeInteger">1</owl:qualifiedCardinality>
			</owl:Restriction>
		</rdfs:subClassOf>
		<rdfs:subClassOf>
			<owl:Restriction>
				<owl:onProperty rdf:resource="&oe2022-iem;hasRelativeHumidityComfortRangeUpperBound"/>
				<owl:onDataRange rdf:resource="&xsd;integer"/>
				<owl:qualifiedCardinality rdf:datatype="&xsd;nonNegativeInteger">1</owl:qualifiedCardinality>
			</owl:Restriction>
		</rdfs:subClassOf>
		<rdfs:label xml:lang="en">occupant</rdfs:label>
		<dct:bibliographicCitation>D. Heinzerling, S. Schiavon, T. Webster, and E. Arens, &apos;Indoor Environmental Quality Assessment models: A literature review and a proposed weighting and classification scheme,&apos; Building and Environment, vol. 70, pp. 210 to 222, 2013.  P. Antoniadou and A. M. Papadopoulos, &apos;Occupants&apos; thermal comfort: State of the art and the prospects of personalized assessment in office buildings,&apos; Energy and Buildings, vol. 153, pp. 136 to 149, 2017.  J. Xie, H. Li, C. Li, J. Zhang, and M. Luo, &apos;Review on occupant-centric thermal comfort sensing, predicting, and controlling,&apos; Energy and Buildings, vol. 226, p. 110392, 2020.</dct:bibliographicCitation>
		<dct:source>&apos;Occupant,&apos; Legal Information Institute. [Online]. Available: https://www.law.cornell.edu/wex/occupant. [Accessed: 22 Sep 2022].</dct:source>
		<skos:definition xml:lang="en">someone that resides or is present in or using a building, vehicle, seat, place, etc., at a given time</skos:definition>
	</owl:Class>
	
	<owl:NamedIndividual rdf:about="&oe2022-iem;Off">
		<rdf:type rdf:resource="&oe2022-iem;ComponentState"/>
		<rdfs:label>off</rdfs:label>
		<skos:definition>condition of not currently being powered</skos:definition>
	</owl:NamedIndividual>
	
	<owl:NamedIndividual rdf:about="&oe2022-iem;On">
		<rdf:type rdf:resource="&oe2022-iem;ComponentState"/>
		<rdfs:label>on</rdfs:label>
		<skos:definition>condition of being currently in operation</skos:definition>
	</owl:NamedIndividual>
	
	<owl:NamedIndividual rdf:about="&oe2022-iem;Open">
		<rdf:type rdf:resource="&oe2022-iem;ComponentState"/>
		<rdfs:label>open</rdfs:label>
		<skos:definition>condition of not being completely closed</skos:definition>
	</owl:NamedIndividual>
	
	<owl:Class rdf:about="&oe2022-iem;Organization">
		<rdfs:subClassOf rdf:resource="&cmns-pts;Party"/>
		<rdfs:label xml:lang="en">organization</rdfs:label>
		<rdfs:seeAlso rdf:resource="https://www.w3.org/TR/vocab-org/#org:Organization"/>
		<skos:definition xml:lang="en">collection of one or more people, or groups of people formed together into a community or other social, commercial or political structure to act, or that is designated to act, towards some purpose, such as to meet a need or pursue collective goals on a continuing basis</skos:definition>
		<skos:example xml:lang="en">This may be a business entity, government, international organization, not-for-profit, academic institution, or other unincorporated and/or informal social organization.</skos:example>
		<cmns-av:adaptedFrom>https://www.iso.org/obp/ui/#iso:std:iso-iec:6523:-1:ed-1:v1:en</cmns-av:adaptedFrom>
	</owl:Class>
	
	<owl:Class rdf:about="&oe2022-iem;OutdoorEnvironment">
		<rdfs:subClassOf rdf:resource="&oe2022-iem;DeltaDefinedEnvironment"/>
		<rdfs:subClassOf rdf:resource="&oe2022-iem;Environment"/>
		<rdfs:label>outdoor environment</rdfs:label>
		<dct:source>&quot;Environment&quot;, ASHRAE Terminology, 2022. [Online] Available: https://terminology.ashrae.org/?term=environment</dct:source>
		<skos:definition>all of the outdoor elements over which a designer has no control and that affect a system and its input or output</skos:definition>
	</owl:Class>
	
	<owl:Class rdf:about="&oe2022-iem;Person">
		<rdfs:subClassOf rdf:resource="&cmns-pts;Party"/>
		<rdfs:label xml:lang="en">person</rdfs:label>
		<skos:definition xml:lang="en">individual human being, with consciousness of self</skos:definition>
		<cmns-av:synonym xml:lang="en">natural person</cmns-av:synonym>
	</owl:Class>
	
	<owl:NamedIndividual rdf:about="&oe2022-iem;Positive">
		<rdf:type rdf:resource="&oe2022-iem;Sign"/>
		<rdfs:label>positive</rdfs:label>
		<skos:definition>plus sign that indicates how attributes affects the environment in a positive way</skos:definition>
	</owl:NamedIndividual>
	
	<owl:Class rdf:about="&oe2022-iem;PowerConsumingComponent">
		<rdfs:subClassOf rdf:resource="&oe2022-iem;RoomComponent"/>
		<rdfs:label>power consuming component</rdfs:label>
		<skos:definition>room component that consumes energy</skos:definition>
	</owl:Class>
	
	<owl:Class rdf:about="&oe2022-iem;Radiator">
		<rdfs:subClassOf rdf:resource="&oe2022-iem;HeatingVentilationAndAirConditioningEquipment"/>
		<rdfs:subClassOf>
			<owl:Restriction>
				<owl:onProperty rdf:resource="&oe2022-iem;isControlledBy"/>
				<owl:onClass rdf:resource="&oe2022-iem;Thermostat"/>
				<owl:qualifiedCardinality rdf:datatype="&xsd;nonNegativeInteger">1</owl:qualifiedCardinality>
			</owl:Restriction>
		</rdfs:subClassOf>
		<rdfs:label>radiator</rdfs:label>
		<dct:bibliographicCitation>D. Heinzerling, S. Schiavon, T. Webster, and E. Arens, &apos;Indoor Environmental Quality Assessment models: A literature review and a proposed weighting and classification scheme,&apos; Building and Environment, vol. 70, pp. 210 to 222, 2013.</dct:bibliographicCitation>
		<dct:source>&quot;Radiator,&quot; Merriam-Webster.com, 2022. [Online]. Available: https://www.merriam-webster.com/dictionary/radiator</dct:source>
		<skos:definition>equipment that can raise the indoor temperature by transferring heat from an internal system into a room</skos:definition>
	</owl:Class>
	
	<owl:NamedIndividual rdf:about="&oe2022-iem;RelativeHumidity">
		<rdf:type rdf:resource="&cmns-qtu;QuantityKind"/>
		<rdfs:label>relative humidity</rdfs:label>
		<skos:definition>ratio of the mole fraction of water vapor to the mole fraction of water vapor saturated at the same temperature and barometric pressure.</skos:definition>
	</owl:NamedIndividual>
	
	<owl:Class rdf:about="&oe2022-iem;ResultantIndoorEnvironment">
		<rdfs:subClassOf rdf:resource="&oe2022-iem;DeltaDefinedEnvironment"/>
		<rdfs:subClassOf rdf:resource="&oe2022-iem;IndoorEnvironment"/>
		<rdfs:label>resultant indoor environment</rdfs:label>
		<skos:definition>a collection of indoor environmental parameters after environmental attributes affect the indoor environment</skos:definition>
	</owl:Class>
	
	<owl:Class rdf:about="&oe2022-iem;Room">
		<rdfs:subClassOf rdf:resource="&cmns-col;Collection"/>
		<rdfs:subClassOf>
			<owl:Restriction>
				<owl:onProperty rdf:resource="&oe2022-iem;hasComponent"/>
				<owl:onClass rdf:resource="&oe2022-iem;RoomComponent"/>
				<owl:minQualifiedCardinality rdf:datatype="&xsd;nonNegativeInteger">0</owl:minQualifiedCardinality>
			</owl:Restriction>
		</rdfs:subClassOf>
		<rdfs:subClassOf>
			<owl:Restriction>
				<owl:onProperty rdf:resource="&oe2022-iem;hasEnvironment"/>
				<owl:onClass rdf:resource="&oe2022-iem;CurrentIndoorEnvironment"/>
				<owl:qualifiedCardinality rdf:datatype="&xsd;nonNegativeInteger">1</owl:qualifiedCardinality>
			</owl:Restriction>
		</rdfs:subClassOf>
		<rdfs:label>room</rdfs:label>
		<dct:bibliographicCitation>D. Heinzerling, S. Schiavon, T. Webster, and E. Arens, &apos;Indoor Environmental Quality Assessment models: A literature review and a proposed weighting and classification scheme,&apos; Building and Environment, vol. 70, pp. 210 to 222, 2013.</dct:bibliographicCitation>
		<dct:source>&quot;Room,&quot; Merriam-Webster.com, 2022. [Online]. Available: https://www.merriam-webster.com/dictionary/room</dct:source>
		<skos:definition>region in a building in which occupant comfort and measurements apply</skos:definition>
	</owl:Class>
	
	<owl:Class rdf:about="&oe2022-iem;RoomComponent">
		<rdfs:subClassOf rdf:resource="&cmns-col;Constituent"/>
		<rdfs:subClassOf>
			<owl:Restriction>
				<owl:onProperty rdf:resource="&oe2022-iem;hasAvailableAction"/>
				<owl:onClass rdf:resource="&oe2022-iem;RoomComponentAction"/>
				<owl:minQualifiedCardinality rdf:datatype="&xsd;nonNegativeInteger">0</owl:minQualifiedCardinality>
			</owl:Restriction>
		</rdfs:subClassOf>
		<rdfs:subClassOf>
			<owl:Restriction>
				<owl:onProperty rdf:resource="&oe2022-iem;hasState"/>
				<owl:onClass rdf:resource="&oe2022-iem;ComponentState"/>
				<owl:qualifiedCardinality rdf:datatype="&xsd;nonNegativeInteger">1</owl:qualifiedCardinality>
			</owl:Restriction>
		</rdfs:subClassOf>
		<rdfs:subClassOf>
			<owl:Restriction>
				<owl:onProperty rdf:resource="&oe2022-iem;isComponentOf"/>
				<owl:onClass rdf:resource="&oe2022-iem;Room"/>
				<owl:qualifiedCardinality rdf:datatype="&xsd;nonNegativeInteger">1</owl:qualifiedCardinality>
			</owl:Restriction>
		</rdfs:subClassOf>
		<rdfs:label>room component</rdfs:label>
		<skos:definition>a constituent part of a room that can be used to alter relevant IEQ parameters</skos:definition>
		<cmns-av:adaptedFrom>&quot;Component,&quot; Merriam-Webster.com, 2022. [Online]. Available: https://www.merriam-webster.com/dictionary/component</cmns-av:adaptedFrom>
	</owl:Class>
	
	<owl:Class rdf:about="&oe2022-iem;RoomComponentAction">
		<rdfs:subClassOf>
			<owl:Restriction>
				<owl:onProperty rdf:resource="&oe2022-iem;causesNewState"/>
				<owl:onClass rdf:resource="&oe2022-iem;ComponentState"/>
				<owl:qualifiedCardinality rdf:datatype="&xsd;nonNegativeInteger">1</owl:qualifiedCardinality>
			</owl:Restriction>
		</rdfs:subClassOf>
		<rdfs:subClassOf>
			<owl:Restriction>
				<owl:onProperty rdf:resource="&oe2022-iem;produces"/>
				<owl:onClass rdf:resource="&oe2022-iem;ResultantIndoorEnvironment"/>
				<owl:qualifiedCardinality rdf:datatype="&xsd;nonNegativeInteger">1</owl:qualifiedCardinality>
			</owl:Restriction>
		</rdfs:subClassOf>
		<rdfs:subClassOf>
			<owl:Restriction>
				<owl:onProperty rdf:resource="&oe2022-iem;isAvailableActionFor"/>
				<owl:onClass rdf:resource="&oe2022-iem;RoomComponent"/>
				<owl:qualifiedCardinality rdf:datatype="&xsd;nonNegativeInteger">1</owl:qualifiedCardinality>
			</owl:Restriction>
		</rdfs:subClassOf>
		<rdfs:label>room component action</rdfs:label>
		<skos:definition>An action to change the state of the room component to alter relevant indoor environment quality parameters</skos:definition>
	</owl:Class>
	
	<owl:Class rdf:about="&oe2022-iem;Sign">
		<rdfs:label>sign</rdfs:label>
		<dct:source>&quot;Sign,&quot; Merriam-Webster.com, 2022. [Online]. Available: https://www.merriam-webster.com/dictionary/sign</dct:source>
		<owl:equivalentClass>
			<owl:Class>
				<owl:oneOf rdf:parseType="Collection">
					<rdf:Description rdf:about="&oe2022-iem;Negative">
					</rdf:Description>
					<rdf:Description rdf:about="&oe2022-iem;Positive">
					</rdf:Description>
				</owl:oneOf>
			</owl:Class>
		</owl:equivalentClass>
		<skos:definition>a fundamental linguistic unit that designates an object or relation or has a purely syntactic function</skos:definition>
	</owl:Class>
	
	<owl:Class rdf:about="&oe2022-iem;SpaceHeater">
		<rdfs:subClassOf rdf:resource="&oe2022-iem;PowerConsumingComponent"/>
		<rdfs:label>space heater</rdfs:label>
		<dct:source>&quot;Space heater,&quot; Merriam-Webster.com, 2022. [Online]. Available: https://www.merriam-webster.com/dictionary/radiator</dct:source>
		<skos:definition>portable appliance that can raise the indoor temperature by heating the air around it</skos:definition>
	</owl:Class>
	
	<owl:NamedIndividual rdf:about="&oe2022-iem;Temperature">
		<rdf:type rdf:resource="&cmns-qtu;QuantityKind"/>
		<rdfs:label>temperature</rdfs:label>
		<dct:source>https://ucum.org/ucum.html#section-Base-Units</dct:source>
		<skos:definition>base quantity kind that is the quantitative measure of the ability of a substance, or more generally of any physical system, to transfer heat energy to another physical system</skos:definition>
		<cmns-av:explanatoryNote>There are three types of temperature scale: those, such as the SI scale, that are defined in terms of the average translational kinetic energy per freely moving microscopic particle, such as atom, molecule, or electron, in a body; those that rely solely on purely macroscopic properties and thermodynamic principles, such as Kelvin&apos;s original definition; and those that are not defined by theoretical principles, but are defined by convenient empirical properties of particular materials.</cmns-av:explanatoryNote>
		<cmns-av:symbol>T</cmns-av:symbol>
	</owl:NamedIndividual>
	
	<owl:Class rdf:about="&oe2022-iem;ThermalComfort">
		<rdfs:subClassOf rdf:resource="&oe2022-iem;IndoorEnvironmentalQuality"/>
		<rdfs:label>thermal comfort</rdfs:label>
		<dct:bibliographicCitation>D. Heinzerling, S. Schiavon, T. Webster, and E. Arens, &apos;Indoor Environmental Quality Assessment models: A literature review and a proposed weighting and classification scheme,&apos; Building and Environment, vol. 70, pp. 210 to 222, 2013.</dct:bibliographicCitation>
		<dct:source>&quot;Thermal comfort&quot;, ASHRAE Terminology, 2022. [Online]. Available: https://terminology.ashrae.org/?entry=thermal%20comfort</dct:source>
		<skos:definition>the condition of mind that expresses satisfaction with the surrounding thermal environment and is assessed by subjective evaluation</skos:definition>
	</owl:Class>
	
	<owl:Class rdf:about="&oe2022-iem;Thermostat">
		<rdfs:subClassOf rdf:resource="&oe2022-iem;NonPowerConsumingComponent"/>
		<rdfs:subClassOf>
			<owl:Restriction>
				<owl:onProperty rdf:resource="&oe2022-iem;controls"/>
				<owl:onClass rdf:resource="&oe2022-iem;HeatingVentilationAndAirConditioningEquipment"/>
				<owl:minQualifiedCardinality rdf:datatype="&xsd;nonNegativeInteger">1</owl:minQualifiedCardinality>
			</owl:Restriction>
		</rdfs:subClassOf>
		<rdfs:subClassOf>
			<owl:Restriction>
				<owl:onProperty rdf:resource="&oe2022-iem;hasState"/>
				<owl:onClass rdf:resource="&oe2022-iem;ThermostatState"/>
				<owl:qualifiedCardinality rdf:datatype="&xsd;nonNegativeInteger">1</owl:qualifiedCardinality>
			</owl:Restriction>
		</rdfs:subClassOf>
		<rdfs:label>thermostat</rdfs:label>
		<dct:bibliographicCitation>J. Xie, H. Li, C. Li, J. Zhang, and M. Luo, &apos;Review on occupant-centric thermal comfort sensing, predicting, and controlling,&apos; Energy and Buildings, vol. 226, p. 110392, 2020.</dct:bibliographicCitation>
		<dct:source>&quot;Thermostat,&quot; Merriam-Webster.com, 2022. [Online]. Available: https://www.merriam-webster.com/dictionary/thermostat</dct:source>
		<skos:definition>heating, ventilation, and air conditioning equipment that can control air conditioning</skos:definition>
	</owl:Class>
	
	<owl:Class rdf:about="&oe2022-iem;ThermostatState">
		<rdfs:subClassOf rdf:resource="&oe2022-iem;ComponentState"/>
		<rdfs:subClassOf>
			<owl:Restriction>
				<owl:onProperty rdf:resource="&cmns-qtu;hasNumericValue"/>
				<owl:onDataRange rdf:resource="&xsd;int"/>
				<owl:qualifiedCardinality rdf:datatype="&xsd;nonNegativeInteger">1</owl:qualifiedCardinality>
			</owl:Restriction>
		</rdfs:subClassOf>
		<rdfs:label>thermostat state</rdfs:label>
		<skos:definition>numeric value at which the thermostat is set</skos:definition>
	</owl:Class>
	
	<owl:NamedIndividual rdf:about="&oe2022-iem;Time">
		<rdf:type rdf:resource="&cmns-qtu;QuantityKind"/>
		<rdfs:label>time</rdfs:label>
		<skos:definition>the measured or measurable period during which an action, process, or condition exists or continues</skos:definition>
	</owl:NamedIndividual>
	
	<owl:Class rdf:about="&oe2022-iem;Window">
		<rdfs:subClassOf rdf:resource="&oe2022-iem;NonPowerConsumingComponent"/>
		<rdfs:label>window</rdfs:label>
		<dct:bibliographicCitation>D. Heinzerling, S. Schiavon, T. Webster, and E. Arens, &apos;Indoor Environmental Quality Assessment models: A literature review and a proposed weighting and classification scheme,&apos; Building and Environment, vol. 70, pp. 210 to 222, 2013.  P. Antoniadou and A. M. Papadopoulos, &apos;Occupants&apos; thermal comfort: State of the art and the prospects of personalized assessment in office buildings,&apos; Energy and Buildings, vol. 153, pp. 136 to 149, 2017.  J. Xie, H. Li, C. Li, J. Zhang, and M. Luo, &apos;Review on occupant-centric thermal comfort sensing, predicting, and controlling,&apos; Energy and Buildings, vol. 226, p. 110392, 2020.</dct:bibliographicCitation>
		<dct:source>&quot;Window,&quot; Merriam-Webster.com, 2022. [Online]. Available: https://www.merriam-webster.com/dictionary/window</dct:source>
		<owl:disjointWith rdf:resource="&oe2022-iem;WindowBlinds"/>
		<skos:definition>room component that can optionally let air flow between inside and outside regions</skos:definition>
	</owl:Class>
	
	<owl:Class rdf:about="&oe2022-iem;WindowBlinds">
		<rdfs:subClassOf rdf:resource="&oe2022-iem;NonPowerConsumingComponent"/>
		<rdfs:label>window blinds</rdfs:label>
		<skos:definition>room component that be open or closed, thereby letting in or blocking light, respectively</skos:definition>
	</owl:Class>
	
	<owl:ObjectProperty rdf:about="&oe2022-iem;causesNewState">
		<rdfs:label>causes new state</rdfs:label>
		<rdfs:range rdf:resource="&oe2022-iem;ComponentState"/>
		<skos:definition>determines the state of the room component</skos:definition>
	</owl:ObjectProperty>
	
	<owl:ObjectProperty rdf:about="&oe2022-iem;controls">
		<rdfs:label>controls</rdfs:label>
		<dct:source>&quot;Control,&quot; Merriam-Webster.com, 2022. [Online]. Available: https://www.merriam-webster.com/dictionary/control</dct:source>
		<owl:inverseOf rdf:resource="&oe2022-iem;isControlledBy"/>
		<skos:definition>to exercise restraining or directing influence over</skos:definition>
	</owl:ObjectProperty>
	
	<owl:DatatypeProperty rdf:about="&oe2022-iem;hasAirQualityValue">
		<rdfs:subPropertyOf rdf:resource="&oe2022-iem;hasEnvironmentAttributeValue"/>
		<rdfs:label>has air quality value</rdfs:label>
		<skos:definition>specifies an actual literal (explicit) values of air quality index</skos:definition>
	</owl:DatatypeProperty>
	
	<owl:DatatypeProperty rdf:about="&oe2022-iem;hasAirSpeedComfortRangeLowerBound">
		<rdfs:subPropertyOf rdf:resource="&oe2022-iem;hasComfortRangeLowerBound"/>
		<rdfs:label>has air speed comfort range lower bound</rdfs:label>
		<skos:definition>indicates a lower bound of a range where an occupant feel comfortable for air speed in an indoor circumstance</skos:definition>
	</owl:DatatypeProperty>
	
	<owl:DatatypeProperty rdf:about="&oe2022-iem;hasAirSpeedComfortRangeUpperBound">
		<rdfs:subPropertyOf rdf:resource="&oe2022-iem;hasComfortRangeUpperBound"/>
		<rdfs:label>has air speed comfort range upper bound</rdfs:label>
		<skos:definition>indicates an upper bound of a range where an occupant feel comfortable for air speed in an indoor circumstance</skos:definition>
	</owl:DatatypeProperty>
	
	<owl:ObjectProperty rdf:about="&oe2022-iem;hasAirSpeedSign">
		<rdfs:subPropertyOf rdf:resource="&oe2022-iem;hasSign"/>
		<rdfs:label>has air speed sign</rdfs:label>
		<skos:definition>indicates how attributes affects the air speed in a positive or negative way</skos:definition>
	</owl:ObjectProperty>
	
	<owl:DatatypeProperty rdf:about="&oe2022-iem;hasAirSpeedValue">
		<rdfs:subPropertyOf rdf:resource="&oe2022-iem;hasEnvironmentAttributeValue"/>
		<rdfs:label>has air speed value</rdfs:label>
		<skos:definition>specifies an actual literal (explicit) values of air speed</skos:definition>
	</owl:DatatypeProperty>
	
	<owl:DatatypeProperty rdf:about="&oe2022-iem;hasAirTemperatureComfortRangeLowerBound">
		<rdfs:subPropertyOf rdf:resource="&oe2022-iem;hasComfortRangeLowerBound"/>
		<rdfs:label>has air temperature comfort range lower bound</rdfs:label>
		<skos:definition>indicates a lower bound of a range where an occupant feel comfortable for air temperature in an indoor circumstance</skos:definition>
	</owl:DatatypeProperty>
	
	<owl:DatatypeProperty rdf:about="&oe2022-iem;hasAirTemperatureComfortRangeUpperBound">
		<rdfs:subPropertyOf rdf:resource="&oe2022-iem;hasComfortRangeUpperBound"/>
		<rdfs:label>has air temperature comfort range upper bound</rdfs:label>
		<skos:definition>indicates an upper bound of a range where an occupant feel comfortable for air temperature in an indoor circumstance</skos:definition>
	</owl:DatatypeProperty>
	
	<owl:ObjectProperty rdf:about="&oe2022-iem;hasAirTemperatureSign">
		<rdfs:subPropertyOf rdf:resource="&oe2022-iem;hasSign"/>
		<rdfs:label>has air temperature sign</rdfs:label>
		<skos:definition>indicates how attributes affects the air temperature in a positive or negative way</skos:definition>
	</owl:ObjectProperty>
	
	<owl:DatatypeProperty rdf:about="&oe2022-iem;hasAirTemperatureValue">
		<rdfs:subPropertyOf rdf:resource="&oe2022-iem;hasEnvironmentAttributeValue"/>
		<rdfs:label>has air temperature value</rdfs:label>
		<skos:definition>specifies an actual literal (explicit) values of ambient temperature</skos:definition>
	</owl:DatatypeProperty>
	
	<owl:ObjectProperty rdf:about="&oe2022-iem;hasAttribute">
		<rdfs:subPropertyOf rdf:resource="&owl;topObjectProperty"/>
		<rdfs:label>has attribute</rdfs:label>
		<owl:inverseOf rdf:resource="&oe2022-iem;isAttributeOf"/>
		<skos:definition>has components that affect the nature of the whole with respect to relevant actors</skos:definition>
	</owl:ObjectProperty>
	
	<owl:ObjectProperty rdf:about="&oe2022-iem;hasAvailableAction">
		<rdfs:label>has available action</rdfs:label>
		<rdfs:range rdf:resource="&oe2022-iem;RoomComponentAction"/>
		<owl:inverseOf rdf:resource="&oe2022-iem;isAvailableActionFor"/>
		<skos:definition>indicates what actions are available for a room component</skos:definition>
	</owl:ObjectProperty>
	
	<owl:DatatypeProperty rdf:about="&oe2022-iem;hasComfortRangeBound">
		<rdfs:label>has comfort range bound</rdfs:label>
		<rdfs:range rdf:resource="&xsd;integer"/>
		<skos:definition>indicates bounds of a range where an occupant feel comfortable in an indoor circumstance</skos:definition>
	</owl:DatatypeProperty>
	
	<owl:DatatypeProperty rdf:about="&oe2022-iem;hasComfortRangeLowerBound">
		<rdfs:subPropertyOf rdf:resource="&oe2022-iem;hasComfortRangeBound"/>
		<rdfs:label>has comfort range lower bound</rdfs:label>
		<skos:definition>indicates a lower bound of a range where an occupant feel comfortable in an indoor circumstance</skos:definition>
	</owl:DatatypeProperty>
	
	<owl:DatatypeProperty rdf:about="&oe2022-iem;hasComfortRangeUpperBound">
		<rdfs:subPropertyOf rdf:resource="&oe2022-iem;hasComfortRangeBound"/>
		<rdfs:label>has comfort range upper bound</rdfs:label>
		<skos:definition>indicates an upper bound of a range where an occupant feel comfortable in an indoor circumstance</skos:definition>
	</owl:DatatypeProperty>
	
	<owl:ObjectProperty rdf:about="&oe2022-iem;hasComponent">
		<rdfs:label>has component</rdfs:label>
		<owl:inverseOf rdf:resource="&oe2022-iem;isComponentOf"/>
		<skos:definition>contains some object within itself, in a semi-permanent capacity</skos:definition>
	</owl:ObjectProperty>
	
	<owl:DatatypeProperty rdf:about="&oe2022-iem;hasDaylightIntensityValue">
		<rdfs:subPropertyOf rdf:resource="&oe2022-iem;hasEnvironmentAttributeValue"/>
		<rdfs:label>has daylight intensity value</rdfs:label>
		<skos:definition>specifies an actual literal (explicit) values of daylight intensity</skos:definition>
	</owl:DatatypeProperty>
	
	<owl:ObjectProperty rdf:about="&oe2022-iem;hasEffect">
		<rdfs:label>has effect</rdfs:label>
		<skos:definition>specify how to achange the parameters of indoor environmental quality</skos:definition>
	</owl:ObjectProperty>
	
	<owl:ObjectProperty rdf:about="&oe2022-iem;hasEnvironment">
		<rdfs:label>has environment</rdfs:label>
		<rdfs:range rdf:resource="&oe2022-iem;Environment"/>
		<skos:definition>indicates the environmental condition that consists of indoor and outdoor environmental parameters</skos:definition>
	</owl:ObjectProperty>
	
	<owl:DatatypeProperty rdf:about="&oe2022-iem;hasEnvironmentAttributeValue">
		<rdfs:label>has environment attribute value</rdfs:label>
		<rdfs:range rdf:resource="&xsd;integer"/>
		<skos:definition>specifies an actual literal (explicit) values of environmental attributes</skos:definition>
	</owl:DatatypeProperty>
	
	<owl:DatatypeProperty rdf:about="&oe2022-iem;hasLowerBound">
		<rdfs:subPropertyOf rdf:resource="&cmns-qtu;hasNumericValue"/>
		<rdfs:label>has lower bound (old)</rdfs:label>
		<skos:definition>indicates a lower bound of a delta bucket for an indoor environmental quality parameter</skos:definition>
	</owl:DatatypeProperty>
	
	<owl:ObjectProperty rdf:about="&oe2022-iem;hasOccupant">
		<rdfs:label>has occupant</rdfs:label>
		<rdfs:domain rdf:resource="&oe2022-iem;Room"/>
		<owl:inverseOf rdf:resource="&oe2022-iem;occupies"/>
		<skos:definition>has as one who resides in, or has as one&apos;s place of business</skos:definition>
	</owl:ObjectProperty>
	
	<owl:ObjectProperty rdf:about="&oe2022-iem;hasPossibleState">
		<rdfs:subPropertyOf rdf:resource="&owl;topObjectProperty"/>
		<rdfs:label>has possible state</rdfs:label>
		<rdfs:domain rdf:resource="&oe2022-iem;RoomComponent"/>
		<rdfs:range rdf:resource="&oe2022-iem;ComponentState"/>
		<owl:inverseOf rdf:resource="&oe2022-iem;isPossibleStateOf"/>
		<skos:definition>has the ability to be in some condition at a point in time</skos:definition>
	</owl:ObjectProperty>
	
	<owl:DatatypeProperty rdf:about="&oe2022-iem;hasRelativeHumidityComfortRangeLowerBound">
		<rdfs:subPropertyOf rdf:resource="&oe2022-iem;hasComfortRangeLowerBound"/>
		<rdfs:label>has relative humidity comfort range lower bound</rdfs:label>
		<skos:definition>indicates a lower bound of a range where an occupant feel comfortable for relative humidity in an indoor circumstance</skos:definition>
	</owl:DatatypeProperty>
	
	<owl:DatatypeProperty rdf:about="&oe2022-iem;hasRelativeHumidityComfortRangeUpperBound">
		<rdfs:subPropertyOf rdf:resource="&oe2022-iem;hasComfortRangeUpperBound"/>
		<rdfs:label>has relative humidity comfort range upper bound</rdfs:label>
		<skos:definition>indicates an upper bound of a range where an occupant feel comfortable for air temperature in an indoor circumstance</skos:definition>
	</owl:DatatypeProperty>
	
	<owl:ObjectProperty rdf:about="&oe2022-iem;hasRelativeHumiditySign">
		<rdfs:subPropertyOf rdf:resource="&oe2022-iem;hasSign"/>
		<rdfs:label>has relative humidity sign</rdfs:label>
		<skos:definition>indicates how attributes affects the relative humidity in a positive or negative way</skos:definition>
	</owl:ObjectProperty>
	
	<owl:DatatypeProperty rdf:about="&oe2022-iem;hasRelativeHumidityValue">
		<rdfs:subPropertyOf rdf:resource="&oe2022-iem;hasEnvironmentAttributeValue"/>
		<rdfs:label>has relative humidity value</rdfs:label>
		<skos:definition>specifies an actual literal (explicit) values of relative humidity</skos:definition>
	</owl:DatatypeProperty>
	
	<owl:ObjectProperty rdf:about="&oe2022-iem;hasSign">
		<rdfs:label>has sign</rdfs:label>
		<rdfs:range rdf:resource="&oe2022-iem;Sign"/>
		<skos:definition>indicates how attributes affects the environment in a positive or negative way</skos:definition>
	</owl:ObjectProperty>
	
	<owl:ObjectProperty rdf:about="&oe2022-iem;hasState">
		<rdfs:subPropertyOf rdf:resource="&owl;topObjectProperty"/>
		<rdfs:label>has state</rdfs:label>
		<rdfs:domain rdf:resource="&oe2022-iem;RoomComponent"/>
		<rdfs:range rdf:resource="&oe2022-iem;ComponentState"/>
		<owl:inverseOf rdf:resource="&oe2022-iem;isStateOf"/>
		<skos:definition>is currently in the condition, referring to objects that have some changeable condition</skos:definition>
	</owl:ObjectProperty>
	
	<owl:DatatypeProperty rdf:about="&oe2022-iem;hasUpperBound">
		<rdfs:subPropertyOf rdf:resource="&cmns-qtu;hasNumericValue"/>
		<rdfs:label>has upper bound (old)</rdfs:label>
		<skos:definition>indicates a upper bound of a delta bucket for an indoor environmental quality parameter</skos:definition>
	</owl:DatatypeProperty>
	
	<owl:ObjectProperty rdf:about="&oe2022-iem;isAttributeOf">
		<rdfs:subPropertyOf rdf:resource="&owl;topObjectProperty"/>
		<rdfs:label>is attribute of</rdfs:label>
		<skos:definition>is a component that affects the nature of the whole with respect to relevant actors</skos:definition>
	</owl:ObjectProperty>
	
	<owl:ObjectProperty rdf:about="&oe2022-iem;isAvailableActionFor">
		<rdfs:label>is available action for</rdfs:label>
		<rdfs:domain rdf:resource="&oe2022-iem;RoomComponentAction"/>
		<skos:definition>indicates what room components have the available actions</skos:definition>
	</owl:ObjectProperty>
	
	<owl:ObjectProperty rdf:about="&oe2022-iem;isComponentOf">
		<rdfs:subPropertyOf rdf:resource="&cmns-col;isPartOf"/>
		<rdfs:label>is component of</rdfs:label>
		<skos:definition>physically exists in the space in a semi-permanent capacity</skos:definition>
	</owl:ObjectProperty>
	
	<owl:ObjectProperty rdf:about="&oe2022-iem;isControlledBy">
		<rdfs:label>is controlled by</rdfs:label>
		<skos:definition>has its behavior determined by</skos:definition>
	</owl:ObjectProperty>
	
	<owl:ObjectProperty rdf:about="&oe2022-iem;isPossibleStateOf">
		<rdfs:subPropertyOf rdf:resource="&owl;topObjectProperty"/>
		<rdfs:label>is possible state of</rdfs:label>
		<skos:definition>can be the condition of a given object at some point in time</skos:definition>
	</owl:ObjectProperty>
	
	<owl:ObjectProperty rdf:about="&oe2022-iem;isQuantifiedBy">
		<rdfs:label>is quantified by</rdfs:label>
		<owl:inverseOf rdf:resource="&oe2022-iem;quatifies"/>
		<skos:definition>is specified by the quantify of the object</skos:definition>
	</owl:ObjectProperty>
	
	<owl:ObjectProperty rdf:about="&oe2022-iem;isStateOf">
		<rdfs:subPropertyOf rdf:resource="&owl;topObjectProperty"/>
		<rdfs:label>is state of</rdfs:label>
		<skos:definition>is currently the condition of</skos:definition>
	</owl:ObjectProperty>
	
	<owl:ObjectProperty rdf:about="&oe2022-iem;occupies">
		<rdfs:subPropertyOf rdf:resource="&owl;topObjectProperty"/>
		<rdfs:label>occupies</rdfs:label>
		<rdfs:range rdf:resource="&oe2022-iem;Room"/>
		<skos:definition>resides in or has as one&apos;s place of business</skos:definition>
	</owl:ObjectProperty>
	
	<owl:ObjectProperty rdf:about="&oe2022-iem;produces">
		<rdfs:label>produces</rdfs:label>
		<skos:definition>causes to have existence</skos:definition>
	</owl:ObjectProperty>
	
	<owl:ObjectProperty rdf:about="&oe2022-iem;quatifies">
		<rdfs:label>quantifies</rdfs:label>
		<skos:definition>specifies the quantify of the object</skos:definition>
	</owl:ObjectProperty>
	
	<owl:Class rdf:about="&cmns-qtu;MeasurementUnit">
		<rdfs:label>measurement unit</rdfs:label>
		<skos:definition>a standarized system of units and measurements</skos:definition>
	</owl:Class>
	
	<owl:Class rdf:about="&cmns-qtu;QuantityKind">
		<rdfs:label>quantity kind</rdfs:label>
		<skos:definition>a measurement  that can be quantified as a numeric value</skos:definition>
	</owl:Class>
	
	<owl:DatatypeProperty rdf:about="&cmns-qtu;hasFactorValue">
		<rdfs:subPropertyOf rdf:resource="&cmns-qtu;hasNumericValue"/>
		<rdfs:label>has factor value</rdfs:label>
		<skos:definition>provides a numeric value for an environmental factor</skos:definition>
	</owl:DatatypeProperty>
	
	<owl:ObjectProperty rdf:about="&cmns-qtu;hasLowerBound">
		<rdfs:label>has lower bound</rdfs:label>
		<skos:definition>specifies the quantity value that is the lower value of a pair of values representing a range</skos:definition>
	</owl:ObjectProperty>
	
	<owl:DatatypeProperty rdf:about="&cmns-qtu;hasNumericValue">
		<rdfs:label>has numeric value</rdfs:label>
		<skos:definition>provides a numeric value for something, with or without a language tag</skos:definition>
	</owl:DatatypeProperty>
	
	<owl:ObjectProperty rdf:about="&cmns-qtu;hasUpperBound">
		<rdfs:label>has upper bound</rdfs:label>
		<skos:definition>specifies the quantity value that is the higher value of a pair of values representing a range</skos:definition>
	</owl:ObjectProperty>
	
	<owl:AllDifferent>
		<owl:distinctMembers rdf:parseType="Collection">
			<rdf:Description rdf:about="&oe2022-iem;Negative">
			</rdf:Description>
			<rdf:Description rdf:about="&oe2022-iem;Positive">
			</rdf:Description>
		</owl:distinctMembers>
	</owl:AllDifferent>
	<owl:AllDisjointClasses>
		<owl:members rdf:parseType="Collection">
			<rdf:Description rdf:about="&oe2022-iem;AirConditioning">
			</rdf:Description>
			<rdf:Description rdf:about="&oe2022-iem;Dehumidifier">
			</rdf:Description>
			<rdf:Description rdf:about="&oe2022-iem;Fan">
			</rdf:Description>
			<rdf:Description rdf:about="&oe2022-iem;Radiator">
			</rdf:Description>
		</owl:members>
	</owl:AllDisjointClasses>
	<owl:AllDisjointClasses>
		<owl:members rdf:parseType="Collection">
			<rdf:Description rdf:about="&oe2022-iem;AirConditioning">
			</rdf:Description>
			<rdf:Description rdf:about="&oe2022-iem;Dehumidifier">
			</rdf:Description>
			<rdf:Description rdf:about="&oe2022-iem;Fan">
			</rdf:Description>
			<rdf:Description rdf:about="&oe2022-iem;Radiator">
			</rdf:Description>
			<rdf:Description rdf:about="&oe2022-iem;SpaceHeater">
			</rdf:Description>
		</owl:members>
	</owl:AllDisjointClasses>
</rdf:RDF>